impl fold_encode_nth_miss

proof/lemma/utils.v
@@ -1,5 +1,5 @@
 Require Import List.
-Import ListNotations.
+Import ListNotations Nat Bool.
 From Minirust.def Require Import utils ty le.
 From Minirust.proof.lemma Require Import le.
 
@@ -7,6 +7,11 @@ Lemma declare_impl {T: Type} (t: T) : exists t', t=t'. exists t. reflexivity. Qe
 
 Ltac declare x Hx obj := destruct (declare_impl obj) as [x Hx].
 Ltac have x obj := destruct (declare_impl obj) as [x _].
+
+Definition contains i (interval: nat * nat) := (
+  (fst interval <=? i) &&
+  (i <? fst interval + snd interval)
+).
 
 Lemma bind_some {T T'} {x: T} {f: T -> option T'} : (Some x >>= f) = f x.
 Proof.
